src/SubstSemantics.v
@@ -1111,7 +1111,10 @@ Proof.
   * inversion H. exists (S x). constructor. auto.
   * inversion H. exists (S x). constructor. auto.
   * inversion H. exists (S (S x)). inversion P2. do 2 constructor; auto.
-  * destruct H. assert (| FSend p :: Fs, e | x ↓) by auto.
+  * destruct H. assert (| FSend1 e :: Fs, e0 | x ↓) by auto.
+    apply term_eval in H as [v [k [Cl H']]]; auto.
+    eapply terminates_step_any_2 in H'. 2: exact H0. inversion H'; subst; try inversion_is_value.
+  * destruct H. assert (| FSend2 p :: Fs, e | x ↓) by auto.
     apply term_eval in H as [v [k [Cl H']]]; auto.
     eapply terminates_step_any_2 in H'. 2: exact H0. inversion H'; subst; try inversion_is_value.
 Unshelve.
@@ -1148,6 +1151,7 @@ Proof.
   * destruct H0. simpl in H0. inversion H0; subst; try inversion_is_value.
     inversion H. subst. inversion H5; subst; try inversion_is_value.
     eexists. eauto.
+  * simpl in H0. destruct H0. inversion H0; try inversion_is_value.
   * simpl in H0. destruct H0. inversion H0; try inversion_is_value.
 Qed.
 
